# ECE374 SP23 HW4

## Contributors

Zhirong Chen (zhirong4)

Ziyuan Chen (ziyuanc3)

<br>

## Problem 1

Solve the following recurrence relations. For parts (a) and (b), give an exact solution. For parts (c) and (d), give an asymptotic one. In both cases, justify your solution.


**(a)** $A(n) = A(n − 1) + 2n + 1; A(0) = 0$

**(b)** $B(n) = B(n − 1) + n(n − 1) − 1; B(0) = 0$

**(c)** $C(n) = C\left(\frac{n}{2}\right) + C\left(\frac{n}{3}\right) + C\left(\frac{n}{6}\right) + n$

**(d)** $D(n) = D\left(\frac{n}{2}\right) + D\left(\frac{n}{3}\right) + D\left(\frac{n}{6}\right) + n^2$

<br>

## Solution

### **(a)** $n^2 + 2n$

$$ \begin{aligned}
A(n) &= A(0) + \sum_{k=1}^{n} (2k + 1) \\
&= 0 + 2\sum_{k=1}^{n} k + \sum_{k=1}^{n} 1 \\
&= 2 \times \frac{n(n + 1)}{2} + n \\
&= n^2 + 2n
\end{aligned} $$

### **(b)** $\frac{1}{3} n^3 - \frac{4}{3} n$

$$ \begin{aligned}
B(n) &= B(0) + \sum_{k=1}^{n} (k(k - 1) - 1) \\
&= 0 + \sum_{k=1}^{n} k^2 - \sum_{k=1}^{n} k - \sum_{k=1}^{n} 1 \\
&= \frac{n(n + 1)(2n + 1)}{6} - \frac{n(n + 1)}{2} - n \\
&= \frac{n(n ^ 2 - 4)}{3} \\
\end{aligned} $$

### **(c)** $O(n \log n)$

```
                    C(n)          ··· n
                  /   |   \
            C(n/2) C(n/3) C(n/6)  ··· m
               ·      ·      ·
               ·      ·      ·
               ·      ·      ·
```

$m = \frac{n}{2} + \frac{n}{3} + \frac{n}{6} = n$

$C(n) = n \times \text{depthOfTree} = O(n \log n)$

### **(d)** $O(n^2)$

```
                    C(n)          ··· n ^ 2
                  /   |   \
            C(n/2) C(n/3) C(n/6)  ··· m
               ·      ·      ·
               ·      ·      ·
               ·      ·      ·
```

$m = \left(\frac{n}{2}\right)^2 + \left(\frac{n}{3}\right)^2 + \left(\frac{n}{6}\right)^2 = \frac{7}{18} n^2$

$C(n) = n^2 \times (1 + \frac{7}{18} + \left(\frac{7}{18}\right)^2 + \cdots + \left(\frac{7}{18}\right)^{\log n}) = O(n^2)$
